galois/network/labels.lean
@@ -1,6 +1,9 @@
 -- author: Ben Sherman
 
 import galois.network.network_monad
+import galois.tactic
+
+universes u v
 
 namespace network
 
@@ -24,6 +27,41 @@ inductive agent_label : Type
   | send_message : remote_name → message_t → agent_label
   | poll : poll_label → agent_label
 
+
+/-- I'm trying to see how the decidable equality tactic
+   might work
+-/
+def send_message_sf : simp_function [remote_name, message_t]
+  agent_label 
+  := agent_label.send_message
+
+lemma send_message_sf_inj :
+  ∀ xs ys, send_message_sf.ap xs = send_message_sf.ap ys → xs = ys
+:= begin
+intros xs ys H, unfold send_message_sf at H,
+dsimp [hlist] at xs ys,
+cases xs with x xs, cases xs with x1 x2,
+cases ys with y ys, cases ys with y1 y2,
+induction x2, induction y2,
+injection H, f_equal, assumption, f_equal,
+assumption,
+end
+
+/-- Decidable equality is straightforward, but currently it's
+    difficult for me to automate.
+-/
+instance agent_label_decidable_eq : decidable_eq agent_label :=
+begin
+intros x y,
+induction x; induction y;
+  try { apply decidable.is_false, contradiction },
+{ apply decidable.is_true, reflexivity },
+{ apply decidable_eq_inj, tactic.interactive.constructor_inj, 
+  assumption, apply_instance },
+{ admit },
+{ admit }
+end
+
 inductive next_state_label : Type 1
   | agent_update : ip → agent_label → next_state_label
 
@@ -34,6 +72,13 @@ inductive agent_does (a : ip) (P : agent_label → Prop) : next_state_label → 
 /-- Indicates that an agent is polling -/
 inductive polls : agent_label → Prop
 | mk : ∀ (l : poll_label), polls (agent_label.poll l)
+
+instance polls_decidable : decidable_pred polls
+:= begin
+intros x, induction x;
+try { solve1 { apply decidable.is_false; intros contra; cases contra } },
+apply decidable.is_true, constructor,
+end
 
 inductive receives (P : poll_receive_label → Prop) : agent_label → Prop
 | mk : ∀ (t : time) (rn : remote_name) (prl : poll_receive_label),
