galois/tactic.lean
@@ -1,4 +1,7 @@
 import .option
+import galois.list.member
+
+universes u v
 
 open tactic lean lean.parser
 open interactive interactive.types expr
@@ -23,8 +26,6 @@ meta def specialize (H : parse texpr) : tactic unit :=
      tactic.clear to_remove,
      tactic.rename n id
 
-universes u v
-
 def congr_arg_f_equal {A : Sort u} {B : Sort v} {f f' : A → B}
   {x x' : A} : f = f' → x = x' → f x = f' x'
 := begin
@@ -33,6 +34,7 @@ end
 
 /-- The analogue of Coq's `f_equal` tactic -/
 meta def f_equal : tactic unit :=
+  tactic.focus1 $
   try (do apply ``(@congr_arg_f_equal),
   tactic.focus [ reflexivity <|> f_equal, try reflexivity ])
 
@@ -47,7 +49,7 @@ meta def apply_in_aux : expr → tactic expr
            `apply_in H e` using this tactic in Lean
  -/
 meta def apply_in (H : parse ident) (e : parse texpr) 
-  : tactic unit := do
+  : tactic unit := focus1 $ do
   e' ← i_to_expr e,
   ty_e ← infer_type e' >>= whnf,
   goal ← apply_in_aux ty_e,
@@ -58,4 +60,79 @@ meta def apply_in (H : parse ident) (e : parse texpr)
   any_goals (tactic.apply He),
   any_goals (do clear [H], rename n H)
 
+end tactic.interactive
+
+/- I'm trying to make a decidable equality tactic -/
+def hlist : list (Type u) → Type (u+1)
+| [] := punit
+| (x :: xs) := x × hlist xs
+
+instance decidable_eq_unit : decidable_eq punit 
+:= begin 
+intros x y, induction x, induction y,
+apply decidable.is_true, reflexivity
+end
+
+def decidable_eq_prod {A : Type u} {B : Type v}
+  (HA : decidable_eq A) (HB : decidable_eq B)
+  : decidable_eq (A × B)
+:= begin
+apply_instance,
+end
+
+namespace hlist
+def decidable_eq_args {xs : list (Type u)} (H : ∀ x : xs.member, decidable_eq (x.value) )
+  : decidable_eq (hlist xs)
+:= begin
+induction xs; simp [hlist],
+apply_instance, apply decidable_eq_prod,
+specialize (H list.member.here), apply H,
+apply ih_1, intros,
+apply (H x.there)
+end
+end hlist
+
+def simp_function : list (Type u) → Type u → Type u
+| [] ret := ret
+| (a :: args) ret := a → simp_function args ret
+
+namespace simp_function
+def ap : ∀ {args : list (Type u)} {ret : Type u}
+  (f : simp_function args ret) (xs : hlist args), ret
+| [] ret f _ := f
+| (a :: args) ret f (x, xs) := ap (f x) xs
+
+end simp_function
+
+lemma decidable_eq_inj {A : Sort u} {B : Sort v} (f : A → B)
+  (f_inj : ∀ x y : A, f x = f y → x = y)
+  (decA : decidable_eq A) : ∀ x y : A, decidable (f x = f y)
+:= begin
+intros x y,
+have H := decA x y, induction H with H H,
+{ apply decidable.is_false, intros contra,
+  apply H, apply f_inj, assumption },
+{ apply decidable.is_true, f_equal, assumption }
+end
+
+lemma decidable_eq_ap {args : list (Type u)} {ret : Type u}
+  (f : simp_function args ret) 
+  (f_inj : ∀ xs ys, f.ap xs = f.ap ys → xs = ys)
+  (dec_args : ∀ x : args.member, decidable_eq (x.value))
+  (xs ys : hlist args)
+  : decidable (f.ap xs = f.ap ys)
+:= begin
+apply decidable_eq_inj, apply f_inj,
+apply hlist.decidable_eq_args dec_args
+end
+
+namespace tactic.interactive
+meta def constructor_inj : tactic unit := do
+  x ← tactic.get_unused_name "x" none,
+  y ← tactic.get_unused_name "y" none,
+  H ← tactic.get_unused_name "H" none,
+  tactic.interactive.intros [x, y, H],
+  Hexpr ← tactic.get_local H,
+  tactic.injection Hexpr,
+  return unit.star
 end tactic.interactive
