galois/list/member.lean
@@ -8,10 +8,12 @@ inductive member {A : Type u} : list A → Type u
 | here : ∀ {x : A} {xs : list A}, member (x :: xs)
 | there : ∀ {x : A} {xs : list A}, member xs → member (x :: xs)
 
-definition get_member {A : Type u} 
+namespace member
+definition value {A : Type u} 
   : ∀ {xs : list A}, member xs -> A
 | (x :: xs) member.here := x
-| (x :: xs) (member.there m) := get_member m
+| (x :: xs) (member.there m) := value m
+end member
 
 definition remove_member {A : Type u}
   : ∀ (xs : list A), member xs → list A
@@ -31,20 +33,26 @@ inductive el_member {A : Type u} : A → list A → Type u
 | here : ∀ {x : A} {xs : list A}, el_member x (x :: xs)
 | there : ∀ {y x : A} {xs : list A}, el_member y xs → el_member y (x :: xs)
 
-def member_to_el_member {A : Type u}
-  : ∀ {xs : list A} (m : member xs), el_member (get_member m) xs
-| (x :: xs) member.here := el_member.here
-| (x :: xs) (member.there m) := el_member.there (member_to_el_member m)
+namespace member
+def to_el_member {A : Type u}
+  : ∀ {xs : list A} (m : member xs), el_member m.value xs
+| (x :: xs) here := el_member.here
+| (x :: xs) (there m) := el_member.there (to_el_member m)
+end member
 
-def member_st_to_member {A : Type u} {P : A → Prop}
+namespace member_st
+def to_member {A : Type u} {P : A → Prop}
   : ∀ {xs : list A}, member_st P xs → member xs
-| ._ (@member_st.here ._ ._ x xs H) := member.here
-| ._ (@member_st.there ._ ._ _ _ m) := member.there (member_st_to_member m)
+| ._ (@here ._ ._ x xs H) := member.here
+| ._ (@there ._ ._ _ _ m) := member.there (to_member m)
+end member_st
 
-def el_member_to_member {A : Type u}
+namespace el_member
+def to_member {A : Type u}
   : ∀ {x : A} {xs : list A}, el_member x xs → member xs
-| ._ .(x :: xs) (@el_member.here ._ x xs) := member.here
-| ._ ._ (@el_member.there ._ _ _ _ m) := member.there (el_member_to_member m)
+| ._ .(x :: xs) (@here ._ x xs) := member.here
+| ._ ._ (@there ._ _ _ _ m) := member.there (to_member m)
+end el_member
 
 inductive void : Type
 
@@ -94,7 +102,7 @@ def check_member {A : Type u} [decidable_eq A]
   (x : A) (xs : list A)
   : option (member xs)
   := match el_member_decide x xs with
-  | (sum.inl m) := some (el_member_to_member m)
+  | (sum.inl m) := some m.to_member
   | (sum.inr _) := none
   end
 
